added all backup files

src/CompilerCFG.v
@@ -16,11 +16,54 @@ Import ListNotations.
 Open Scope list_scope.
 Open Scope string_scope.
 
-Definition empty_block : block dtyp :=
+
+
+Fixpoint eqb s1 s2 : bool :=
+ match s1, s2 with
+ | EmptyString, EmptyString => true
+ | String c1 s1', String c2 s2' => Ascii.eqb c1 c2 && eqb s1' s2'
+ | _,_ => false
+ end.
+
+Fixpoint is_present (s : string) (l : list string) (b : bool) : bool :=
+  match l with
+  | h::tail => is_present s tail (orb b (eqb h s))
+  | [] => b
+  end.
+
+Fixpoint extract_vars (p : Ast.stmt) (l : list string) : list string :=
+  match p with
+  | Skip => l
+  | Assign x e => if (is_present x l false) then l else (x::l) 
+  | Seq s1 s2 => let l1 := (extract_vars s1 l) in (extract_vars s2 l1)
+  end.
+
+
+Definition gen_alloc (x:string) : instr_id * instr dtyp :=
+  (IId (Name x), (INSTR_Alloca (DTYPE_I 32%N) None None)).
+
+Definition gen_allocs (p : Ast.stmt) : code dtyp :=
+  let var_list := extract_vars p [] in
+    map gen_alloc var_list.
+  
+
+
+Definition gen_code (p : Ast.stmt) : code dtyp :=
+  match p with
+  | Skip => nil
+  | Assign x v => match v with 
+                  | Lit n => [(IVoid 0%Z, (INSTR_Store false ((DTYPE_I 32%N), (EXP_Integer (n))) (DTYPE_Pointer, (EXP_Ident (ID_Local (Name x)))) None))]
+                  end
+  | _ => nil
+  end.
+
+
+
+Definition empty_block (c : code dtyp) : block dtyp :=
     {|
       blk_id    := (Anon 0%Z);
       blk_phis  := nil;
-      blk_code  := nil;
+      blk_code  := c;
       blk_term  := TERM_Ret ((DTYPE_I 32%N), (EXP_Integer (1)%Z));
       blk_comments := None
     |}.
@@ -34,7 +77,7 @@ Definition empty_cfg (b : block dtyp) : cfg dtyp :=
 
 
 Definition compile_cfg (p : Ast.stmt) : cfg dtyp :=
-   empty_cfg empty_block.
+   empty_cfg (empty_block (app (gen_allocs p) (gen_code p))).
 
   
 
