src/CorrectnessTop.v
@@ -1,17 +1,18 @@
 From ASL Require Import
-  Ast Denotation CompilerCFG CorrectnessCFG AslFacts.
+  Ast Denotation CompilerCFG CorrectnessCFG AslFacts Utils.
+
+From Coq Require Import
+ZArith List String Classes.RelationClasses.
+
 
 From Vellvm Require Import
-  Semantics Syntax TopLevel Theory Utils.PropT. 
+  Semantics Syntax TopLevel Theory Utils.PropT  Utils.AListFacts Numeric.Integers Handlers.MemoryTheory Utilities. 
 
 From ITree Require Import
   ITree ITreeFacts KTree KTreeFacts Events.StateFacts Events.MapDefaultFacts Events.StateFacts. 
 
 From ExtLib Require Import
 RelDec Tactics.
-
-From Coq Require Import
-ZArith List String Classes.RelationClasses.
 
 Import ITreeNotations.
 Import ListNotations.
@@ -20,10 +21,18 @@ Import SemNotations.
 Open Scope list_scope.
 Open Scope string_scope.
 
-Definition Renv (g_asl : Denotation.env) (g_llvm : global_env) (l_llvm : local_env) (m_llvm : memory_stack) : Prop :=
-true = true.
+Definition alist_In_uint32 {K R RD_K} k m v :=
+  @FMapAList.alist_find K R RD_K Z k m = Some (trim_int_u32 v)%Z.
 
-Definition eutt_inv {R1 R2} (r1 : R1) (r2 : R2) : Prop := true = true.
+Definition Renv (env_asl : Denotation.env) (g_llvm : global_env) (l_llvm : local_env) (m_llvm : memory_stack) : Prop :=
+forall k v, alist_In_uint32 k env_asl v <-> (get_val g_llvm l_llvm m_llvm k) =  Some (trim_int_u32 v). 
+
+Definition eutt_inv (r1 : (Denotation.env * unit)) (r2 : memory_stack * (local_env * (global_env * uvalue))) : Prop :=
+let asl_env := fst r1 in
+let m_llvm := fst r2 in
+let l_llvm := fst (snd r2) in
+let g_llvm := fst (snd (snd r2)) in
+  Renv asl_env g_llvm l_llvm m_llvm.
 
 Definition bisimilar (t1 : itree (ImpState +' CallE +' PickE +' UBE +' DebugE +' FailureE) unit) (t2 : itree (instr_E) uvalue)  :=
   forall g_llvm l_llvm m_llvm g_asl,
@@ -35,6 +44,179 @@ Definition bisimilar (t1 : itree (ImpState +' CallE +' PickE +' UBE +' DebugE +'
 Definition TT {A B}: A -> B -> Prop  := fun _ _ => True.
   Hint Unfold TT: core.
 
+From Coq Require Import Lia.
+
+
+Lemma z_is_z : forall z, (0 <= z <= Int32.max_unsigned)%Z -> Int32.unsigned (Int32.repr z) = z.
+Proof.
+  intros.
+  destruct z.
+  + auto.
+  + apply Int32.unsigned_repr. auto.
+  + destruct H. destruct H. auto.
+Qed.
+
+
+(* Lemma uvalue_eq:
+  forall (u : uvalue) (v : Z),
+    match u with
+    | UVALUE_I32 i => Some (Int32.intval i)
+    | _ => None
+    end = Some (Int32.intval (Int32.repr v)) ->
+    u = UVALUE_I32 (Int32.repr v).
+Proof.
+  intros.
+  destruct u; try discriminate.
+  apply int32_from_uvalue_eq.
+Qed.
+
+Lemma test : forall u v, match u with
+| UVALUE_I32 i => Some (Int32.intval i)
+| _ => None
+end = Some (Int32.intval (Int32.repr v)) -> u = UVALUE_I32 (Int32.repr v).
+Proof.
+   intros.
+  remember (UVALUE_I32 (Int32.repr v)) as u_repr_v.
+  assert (Hdec : {u = u_repr_v} + {u <> u_repr_v}) by apply uvalue_eq_dec.
+  From Coq Require Import Program.Equality.
+  dependent destruction Hdec.
+  - assumption.
+  - exfalso. (* derive a contradiction *)
+    destruct u; try discriminate H.
+    + inversion H. subst. apply n. reflexivity.
+       *)
+
+Lemma test : forall l_llvm m_llvm m x v, match FMapAList.alist_find (Name x) (FMapAList.alist_add (Name x) (UVALUE_Addr (next_logical_key m_llvm, 0%Z)) l_llvm) with
+            | Some (UVALUE_Addr ptr) =>
+                match read m ptr (DTYPE_I 32) with
+                | inr (UVALUE_I32 i) => Some (Int32.unsigned i)
+                | _ => None
+                end
+            | _ => None
+            end = Some (trim_int_u32 v) <-> read m (next_logical_key m_llvm, 0%Z) (DTYPE_I 32) = inr (UVALUE_I32 (Int32.repr v)).
+Proof.
+  split.
+  + intros.
+    rewrite alist_find_add_eq in H.
+    apply correct_int_read in H.
+    auto.
+  + intros.
+    rewrite alist_find_add_eq.
+    apply correct_int_read.
+    auto.
+Qed.
+
+Lemma read_new_in_memstack : forall m x z v,
+read (mem_stack_add m x z) (next_logical_key m, 0%Z) (DTYPE_I 32) =
+            inr (UVALUE_I32 (Int32.repr v)) ->
+Int32.repr v = Int32.repr z.
+Proof.
+  intros.
+  unfold mem_stack_add in H. simpl in H.
+  Arguments add_all_index : simpl never.
+  Arguments serialize_dvalue : simpl never.
+  unfold write in H. 
+  rewrite get_logical_block_add_to_frame in H. 
+  rewrite get_logical_block_of_add_logical_block in H.
+  unfold read in H.
+  simpl in H.
+  rewrite get_logical_block_of_add_logical_block in H.
+  unfold read_in_mem_block in H.
+  rewrite deserialize_serialize in H.
+  + simpl in H. injection H as Heq. rewrite extract_intval in Heq. rewrite extract_intval in Heq.
+    pose proof trim_int_u32_inrange.
+
+    unfold trim_int_u32 in Heq. auto.
+
+  assert (write
+          (add_to_frame
+             (add_logical_block (next_logical_key m) (make_empty_logical_block (DTYPE_I 32)) m)
+             (next_logical_key m)) (next_logical_key m, 0%Z) (DVALUE_I32 (Int32.repr z)) = inr empty_memory_stack).
+  {
+    unfold write.
+    rewrite get_logical_block_add_to_frame. 
+    rewrite get_logical_block_of_add_logical_block .
+    Arguments add_all_index : simpl never.
+    Arguments serialize_dvalue : simpl never.
+    simpl make_empty_logical_block.
+    simpl.
+    
+  }
+  unfold write in H.
+
+(* We need to prove that if every element holds Renv, and we add a new variable called "x" with value z, it will still hold.*)
+Lemma Renv_write_local:
+    forall (x : string) (z : Z) (env_asl : env) (g_llvm : global_env) (l_llvm : local_env) (m_llvm : memory_stack) ,
+      Renv env_asl g_llvm l_llvm m_llvm ->
+      Renv (FMapAList.alist_add x z env_asl) g_llvm (FMapAList.alist_add (Name x) (UVALUE_Addr (next_logical_key m_llvm, 0%Z)) l_llvm)
+      (mem_stack_add m_llvm x z).
+  Proof.
+    intros x z env_asl g_llvm l_llvm m_llvm H0 k v.
+    unfold Renv, get_val.
+    split.
+    (*First, we need to ensure that every variable-value pair inside env_asl, implies it's also in llvm memory.*)
+    + destruct (String.eqb_spec k x).
+      (* We analyze the case where the variable added was in the Renv relationship before, so its being overwritten.*)
+      - subst.
+        unfold alist_In_uint32.
+        intros.
+        rewrite alist_find_add_eq in H.
+        assert (0 <= z <= Int32.max_unsigned)%Z. { 
+          inversion H.
+          apply trim_int_u32_inrange.
+        }
+        destruct H.
+        rewrite alist_find_add_eq .
+        unfold read. simpl.
+        unfold mem_stack_add.
+        simpl.
+        unfold write.
+        rewrite get_logical_block_of_add_to_frame .
+        rewrite get_logical_block_of_add_logical_block.
+        Arguments add_all_index : simpl never.
+        Arguments serialize_dvalue : simpl never.
+        simpl get_logical_block.
+        rewrite get_logical_block_of_add_logical_block.
+        unfold read_in_mem_block.
+        rewrite deserialize_serialize; try constructor.
+        simpl. f_equal. apply z_is_z; auto.
+      - 
+      (* We analyze the case where the variable added is new*)
+        unfold alist_In_uint32.
+        intros.
+        assert (FMapAList.alist_find k (FMapAList.alist_add x z env_asl) = FMapAList.alist_find k env_asl). {
+          apply alist_find_neq . auto.
+        }
+        rewrite H1 in H.
+        unfold Renv in H0.
+        unfold alist_In_uint32 in H0.
+        unfold get_val in H0.
+        apply H0 in H.
+        rewrite alist_find_neq.
+        -- destruct (FMapAList.alist_find (Name k) l_llvm); try discriminate.
+           destruct u; try discriminate.
+           unfold trim_int_u32.
+           unfold Int32.unsigned .
+           unfold trim_int_u32 in H.
+           unfold Int32.unsigned in H.
+           apply correct_int_read.
+           apply correct_int_read in H.
+           pose proof same_read_mem_stack_add.
+           auto.
+        -- (* We prove that k <> x -> Name k <> Name x *)
+           unfold not.
+           intros H'.
+           inversion H'.
+           contradiction.
+
+   + intros Mem_value.
+     unfold alist_In_uint32.
+     destruct (String.eqb_spec k x).
+     - subst.
+       rewrite alist_find_add_eq. 
+       apply test in Mem_value.
+
+       
 
 Theorem compiler_correct (s:stmt) :
   bisimilar (denote_asl s) (denote_cfg (compile_cfg s)).
@@ -46,11 +228,51 @@ Proof.
     unfold denote_cfg. simpl.
     unfold CompilerCFG.empty_block.
     rewrite simpl_block.
+    rewrite denote_code_nil.
+    rewrite bind_ret_.
     rewrite bind_ret_.
     rewrite interp_cfg3_ret.
     rewrite interp_asl_ret.
     red. apply eqit_Ret.
+    unfold eutt_inv.
     auto.
   }
+  +unfold denote_cfg. simpl.
+    unfold CompilerCFG.empty_block.
+    destruct e.
+    rewrite simpl_block.
+    rewrite bind_bind.
+    setoid_rewrite bind_ret_.
+    unfold gen_alloc.
+    rewrite denote_code_cons.
+    rewrite interp_cfg3_bind.
+    setoid_rewrite denote_code_singleton.
+    rewrite simpl_alloca_assign.
+    rewrite bind_ret_.
+    rewrite interp_cfg3_ret.
+    rewrite interp_asl_SetVar.
+    red. apply eqit_Ret.
+    unfold eutt_inv.
+    simpl.
+    
+
+    unfold Renv.
+    unfold Renv in H.
+
+    
+
+    rewrite <- H.
+    rewrite Renv_get_val_add.
+
+
+    assert(FMapAList.alist_find (Name k) (FMapAList.alist_add (Name x) (UVALUE_Addr (next_logical_key m_llvm, 0%Z)) l_llvm) = Some (UVALUE_Addr ptr)).
+    {
+
+    }
+    rewrite alist_In_add_eq.
+    simpl.
+
+
+
 
   
