src/Utils.v
@@ -1,12 +1,25 @@
 From Vellvm Require Import
-  Numeric.Integers Handlers Syntax Semantics.
+  Numeric.Integers Handlers Syntax Semantics Theory.
 
 From Coq Require Import
   String ZArith.
 
+From ASL Require Import CorrectnessCFG.
+
 Require Import ExtLib.Structures.Maps.
 
-(*Get the Z value of a variable name X in the memory*)
+Definition trim_int_u32 (i: Z) : Z :=
+  Int32.unsigned (Int32.repr i).
+
+Lemma trim_int_u32_inrange :
+  forall i, (0 <= (trim_int_u32 i) <= Int32.max_unsigned)%Z.
+Proof.
+  intros.
+  unfold trim_int_u32.
+  apply Int32.unsigned_range_2.
+Qed.
+
+(* Get the Z value of a variable name X in the memory *)
 Definition get_val (g: global_env) (l: local_env) (m: memory_stack) (x: string) : option Z :=
   let addr := FMapAList.alist_find (Name x) l
   in match addr with 
@@ -15,9 +28,261 @@ Definition get_val (g: global_env) (l: local_env) (m: memory_stack) (x: string) 
         match val with
           | inl _ => None
           | inr v => match v with
-                      | UVALUE_I32 i => Some (Int32.unsigned (i))
+                      | UVALUE_I32 i => Some (Int32.unsigned (i))%Z
                       | _ => None
                      end
         end
     | _ => None
   end.
+
+
+(*If I read a value in m and then I allocate a new block, the value after reading it is the same: *)
+Lemma read_after_alloc: forall m m1 ptr ptr' v, 
+read m ptr (DTYPE_I 32) = inr v ->
+allocate m (DTYPE_I 32%N) = inr (m1, ptr') ->
+read m1 ptr (DTYPE_I 32) = inr v.
+Proof.
+  intros.
+  apply can_read_allocated in H as alloc_succ.
+  pose proof freshly_allocated_different_blocks as diff_ptrs.
+  specialize diff_ptrs with (1 := H0) (2 := alloc_succ).
+
+  unfold allocate in H0. simpl in H0. injection H0 as m1_def.
+  subst m1. unfold read.
+  rewrite get_logical_block_of_add_to_frame.
+  simpl.
+
+  unfold read in H.
+  simpl in H.
+
+  assert ((fst ptr) <> (next_logical_key m)). { assert (next_logical_key m = fst ptr'). { rewrite <- H0. auto. } rewrite H1. auto. }
+  rewrite get_logical_block_of_add_logical_block_neq; auto.
+Qed.
+
+
+(*If I read a value in m and then I allocate a new block and write to it, the value after reading again in the new stack, is the same*)
+Lemma read_after_alloc_write: forall m m1 m2 ptr ptr' z v, 
+read m ptr (DTYPE_I 32) = inr (UVALUE_I32 v) ->
+allocate m (DTYPE_I 32%N) = inr (m1, ptr') ->
+write m1 ptr' (DVALUE_I32 (Int32.repr z))  = inr m2 ->
+read m2 ptr (DTYPE_I 32) = inr (UVALUE_I32 v) .
+Proof.
+  intros.
+
+  pose proof read_after_alloc.
+  specialize H2 with (1 := H) (2 := H0).
+
+  pose proof write_different_blocks.
+
+  specialize H3 with (1 := H1) (2 := H2).
+
+  (* First I need to demonstrate that ptr <> ptr'*)
+  (* To do that, I need to demonstrate that a succesful reading implies that the ptr has been previously allocated*)
+  apply can_read_allocated in H as alloc_succ.
+  pose proof freshly_allocated_different_blocks as diff_ptrs.
+  specialize diff_ptrs with (1 := H0) (2 := alloc_succ).
+
+  specialize H3 with (1 := diff_ptrs).
+
+  assert (uvalue_to_dvalue (UVALUE_I32 v) = inr (DVALUE_I32 v)); auto.
+
+  specialize H3 with (1 := H4).
+
+  assert (dvalue_has_dtyp (DVALUE_I32 v) (DTYPE_I 32)). { constructor. }
+
+  specialize H3 with (1 := H5).
+
+  assert (dvalue_has_dtyp (DVALUE_I32 (Int32.repr z))  (DTYPE_I 32)). { constructor. }
+
+  specialize H3 with (1 := H6).
+  
+  auto.
+Qed.
+
+Lemma same_read_mem_stack_add : 
+forall m x z ptr v, read m ptr (DTYPE_I 32) = inr (UVALUE_I32 v) -> read (mem_stack_add m x z) ptr (DTYPE_I 32) = inr (UVALUE_I32 v).
+Proof.
+  intros.
+  pose read_after_alloc_write.
+
+  pose (m1 := add_to_frame (add_logical_block (next_logical_key m) (make_empty_logical_block (DTYPE_I 32)) m) (next_logical_key m)).
+  pose (ptr' := ((next_logical_key m), 0%Z)).
+
+
+  specialize e with (ptr' := ptr') (z := z) (ptr := ptr)  (m := m) (m1 := m1) (m2 := (mem_stack_add m x z)) (v := v) .
+
+  assert (allocate m (DTYPE_I 32) = inr (m1, ptr')). { 
+    subst m1.
+    subst ptr'.
+    auto.
+  }
+
+  assert (write m1 ptr' (DVALUE_I32 (Int32.repr z)) = inr (mem_stack_add m x z) ). {
+    subst m1.
+    subst ptr'.
+    unfold mem_stack_add.
+    unfold allocate.
+    simpl.
+    unfold write.
+    repeat rewrite get_logical_block_add_to_frame .
+    repeat rewrite get_logical_block_of_add_logical_block .
+    simpl.
+    reflexivity.
+  }
+
+    auto.
+
+Qed.
+
+
+Lemma uvalue_eq_int32:
+  forall (a b : int32),
+    UVALUE_I32 a = UVALUE_I32 b ->
+    a = b.
+Proof.
+  intros a b H.
+  pose proof (uvalue_eq_dec (u1 := UVALUE_I32 a) (u2 := UVALUE_I32 b) ) as Hdec.
+  destruct Hdec.
+  - inversion e. reflexivity.
+  - contradiction.
+Qed.
+
+
+Lemma intval_eq_intval : forall a b, Int32.intval a = Int32.intval b -> a = b.
+Proof.
+  intros.
+  destruct a; destruct b.
+  simpl in H.
+  apply Int32.mkint_eq.
+  auto.
+Qed.
+
+
+Lemma correct_int_read : forall m ptr (i:int32), match read m ptr (DTYPE_I 32) with
+                    | inr (UVALUE_I32 i) => Some (Int32.intval i)
+                    | _ => None
+                    end = Some (Int32.intval i) <-> read m ptr (DTYPE_I 32) = inr (UVALUE_I32 i).
+Proof.
+  split.
+  + intros.
+    destruct read; try discriminate;
+    destruct u eqn:Test; try discriminate.
+    f_equal.
+    inversion H.
+    apply intval_eq_intval in H1.
+    rewrite H1.
+    reflexivity.
+  + intros.
+    destruct read; try discriminate.
+    destruct u eqn:Test; try discriminate.
+    inversion H.
+    f_equal.
+Qed.
+
+Lemma extract_intval : forall z,
+  match Int32.repr z with
+  | {| Int32.intval := intval |} => intval
+  end = trim_int_u32 z.
+Proof.
+  intros z.
+  pose proof trim_int_u32_inrange.
+  specialize H with (i:= z).
+
+  destruct Int32.repr eqn:Deq.
+  unfold trim_int_u32.
+  unfold Int32.unsigned. auto.
+  destruct (Int32.repr z) eqn:Deq2.
+  simpl.
+  inversion Deq.
+  reflexivity.
+Qed.
+
+(* 
+Lemma same_mem : forall g l m x s v z, get_val g l m x = Some v -> get_val g l (mem_stack_add m s z) x = Some v.
+Proof.
+  intros.
+  unfold get_val.
+  unfold get_val in H.
+  assert (forall m s z ptr v, read m ptr (DTYPE_I 32) = inr (UVALUE_I32 v) -> read (mem_stack_add m s z) ptr (DTYPE_I 32) = inr (UVALUE_I32 v)). {
+     intros.
+     unfold mem_stack_add.
+
+
+(* If I retrieve some value from a variable x, that value is preserved even if I add more blocks. *)
+Lemma same_mem : forall g l m x s v z, get_val g l m x = Some v -> get_val g l (mem_stack_add m s z) x = Some v.
+Proof.
+  intros.
+  unfold get_val.
+  unfold get_val in H.
+  assert (forall m s z ptr dv, read m ptr (DTYPE_I 32) = inr dv -> read (mem_stack_add m s z) ptr (DTYPE_I 32) = inr dv). {
+    intros.
+    pose proof write_different_blocks .
+    unfold mem_stack_add.
+    simpl.
+    assert (exists m2, write (add_to_frame (add_logical_block (next_logical_key m0) (make_empty_logical_block (DTYPE_I 32)) m0) (next_logical_key m0)) (next_logical_key m0, 0%Z) (DVALUE_I32 (Int32.repr z0)) = inr m2).
+    {
+      assert (dvalue_has_dtyp (DVALUE_I32 (Int32.repr z0)) (DTYPE_I 32)). { constructor. }
+      assert (dtyp_fits (add_to_frame (add_logical_block (next_logical_key m0) (make_empty_logical_block (DTYPE_I 32)) m0) (next_logical_key m0)) (next_logical_key m0, 0%Z) (DTYPE_I 32)). {
+        unfold dtyp_fits. simpl. exists 8. simpl. rewrite get_logical_block_add_to_frame . rewrite get_logical_block_of_add_logical_block . unfold make_empty_logical_block. simpl. exists (make_empty_mem_block (DTYPE_I 32)). exists None. auto.
+        assert ((8 <= 8)%Z). { reflexivity.     } auto.
+      }
+      pose proof write_succeeds.
+      apply (H4 (add_to_frame (add_logical_block (next_logical_key m0) (make_empty_logical_block (DTYPE_I 32)) m0)
+       (next_logical_key m0)) (DVALUE_I32 (Int32.repr z0)) (DTYPE_I 32) (next_logical_key m0, 0%Z)); auto.
+    }
+    simpl.
+
+    assert (write (add_to_frame (add_logical_block (next_logical_key m0) (make_empty_logical_block (DTYPE_I 32)) m0) (next_logical_key m0))
+      (next_logical_key m0, 0%Z) (DVALUE_I32 (Int32.repr z0)) = Some (LBlock sz bytes cid)).
+
+
+
+    
+  }
+
+  unfold mem_stack_add.
+
+From Coq Require Import Lia.
+
+Lemma test : forall i, (0 <= Int32.unsigned i <= Int32.max_unsigned)%Z -> (0 <= (Int32.unsigned (i)) / 8 <= Int32.max_unsigned)%Z.
+Proof.
+  destruct i.
+  simpl. destruct intval.
+  - auto.
+  - assert (forall p, (Z.pos p / 8 < Z.pos p)%Z). {
+      intros.
+      apply Z_div_lt.
+        + lia.
+        + lia.
+    }
+    assert (forall p, (0 <= Z.pos p / 8)%Z). {
+      intros.
+      apply Z_div_pos.
+      + lia.
+      + lia.
+    }
+    intros.
+    specialize (H p) as H_p.
+    specialize (H0 p) as H0_p.
+    clear H H0 intrange.
+    assert ((0 <= Z.pos p / 8 < Z.pos p)%Z). {
+      auto.
+    }
+    lia.
+  - lia.
+Qed. *)
+
+Lemma get_val_inrange : forall g l m x v,
+  get_val g l m x = Some v -> (0 <= v <= Int32.max_unsigned)%Z.
+Proof.
+  intros.
+  unfold get_val in H.
+  simpl in H.
+  destruct (FMapAList.alist_find (Name x) l) eqn:H1; try congruence.
+  destruct u eqn:H2; try congruence.
+  destruct (read m a (DTYPE_I 32)) eqn:H3; try congruence.
+  destruct u0 eqn:H4; try congruence.
+  inversion H.
+  pose proof Int32.unsigned_range_2.
+  auto.
+Qed.
