src/AslFacts.v
@@ -20,12 +20,45 @@ Import SemNotations.
 Open Scope list_scope.
 Open Scope string_scope.
 
-Lemma interp_asl_ret : forall (g:env) (E:Type->Type) x, interp_asl (E:=E) (A:=unit) (Ret x) g ≈ Ret (g, x).
+Lemma interp_asl_ret : forall (g:env) (E:Type->Type) (A:Type) x, interp_asl (E:=E) (A:=A) (Ret x) g ≈ Ret (g, x).
 Proof.
-  intros; unfold ℑ3.
+  intros.
   unfold interp_asl.
   rewrite unfold_interp. simpl.
   unfold MapDefault.interp_map. cbn.
   rewrite interp_state_ret .
+  reflexivity.
+Qed.
+
+
+Lemma interp_asl_SetVar : forall x g v (E:Type->Type),
+    interp_asl (E:=E) (trigger (SetVar x v)) g ≈ Ret (FMapAList.alist_add x v g, tt).
+Proof.
+  intros.
+  unfold interp_asl. simpl.
+  rewrite unfold_interp. simpl. cbn. simpl.
+  unfold resum, ReSum_id, id_, Id_IFun. 
+  unfold cat, handle_ImpState. cbn. unfold Cat_Handler. simpl. unfold Handler.cat. rewrite unfold_interp. simpl. unfold subevent. unfold resum, ReSum_id, id_, Id_IFun.
+  setoid_rewrite interp_ret.
+  unfold inl_.
+  unfold Inl_sum1_Handler. 
+  unfold Handler.inl_.
+  unfold Handler.htrigger.
+  rewrite bind_trigger.
+  unfold MapDefault.interp_map. simpl.
+  rewrite bind_vis_. simpl.
+  rewrite interp_state_vis . simpl.
+  unfold MapDefault.handle_map. simpl.
+  unfold case_. simpl.
+  unfold Case_sum1.
+  unfold case_sum1.
+  setoid_rewrite bind_tau_.
+  setoid_rewrite bind_ret_.
+  unfold fst. simpl.
+  setoid_rewrite bind_ret_.
+  setoid_rewrite interp_state_tau  .
+  setoid_rewrite interp_state_tau  .
+  setoid_rewrite interp_state_ret . simpl.
+  repeat rewrite tau_eutt.
   reflexivity.
 Qed.
