src/Ast.v
@@ -3,14 +3,11 @@ From Coq Require Import
 
 Local Open Scope string_scope.
 
-Definition var : Set := string.
-
 Inductive expr : Type :=
-| Var (_ : var)
 | Lit (_ : Z).
 
 Inductive stmt : Type :=
-| Assign (x : var) (e : expr)    
+| Assign (x : string) (e : expr)    
 | Seq    (a b : stmt)           
 | Skip                         
 .
