src/Correctness.v
@@ -1,0 +1,537 @@
+
+From Vellvm Require Import
+Semantics Syntax TopLevel Theory Utils.PropT. 
+
+From ITree Require Import
+  ITree ITreeFacts KTree KTreeFacts Events.StateFacts Events.State.
+
+From ExtLib Require Import
+RelDec Tactics.
+
+From Coq Require Import
+ZArith List String Classes.RelationClasses.
+
+Import ITreeNotations.
+Import ListNotations.
+Import SemNotations.
+
+Ltac simpl_iter :=
+  unfold CategoryOps.iter, Iter_Kleisli, Basics.iter, MonadIter_itree.
+
+Open Scope list_scope.
+Open Scope string_scope.
+
+
+Definition e_prog :=
+TLE_Definition {|
+  df_prototype := {|dc_name := (Name "main");
+                    dc_type := (TYPE_Function (TYPE_I 32%N) []);
+                    dc_param_attrs := ([], []);
+                    dc_linkage := None;
+                    dc_visibility := None;
+                    dc_dll_storage := None;
+                    dc_cconv := None;
+                    dc_attrs := [];
+                    dc_section := None;
+                    dc_align := None;
+                    dc_gc := None|};
+  df_args := [];
+  df_instrs := (
+                {|
+                  blk_id := (Name "entry");
+                  blk_phis := [];
+                  blk_code := [];
+                  blk_term := TERM_Ret ((TYPE_I 32%N), (EXP_Integer (1)%Z));
+                  blk_comments := None
+                |}
+                , nil (A:=block typ))
+                |}.
+
+Check e_prog.
+Check mcfg_of_tle.
+
+
+Definition e_test : itree L0 uvalue :=
+ denote_vellvm (DTYPE_I 32%N) "main" [] (convert_types (mcfg_of_tle [e_prog])). 
+
+Theorem empty_env : build_global_environment (convert_types (mcfg_of_tle [e_prog])) ≈ r <- trigger (Alloca DTYPE_Pointer);; trigger (GlobalWrite (Name "main") r);; Ret tt.
+Proof.
+unfold build_global_environment. simpl.
+unfold initialize_globals. simpl.
+unfold allocate_globals. simpl.
+setoid_rewrite bind_ret_.
+setoid_rewrite translate_ret.
+repeat setoid_rewrite bind_ret_.
+unfold allocate_declarations. unfold allocate_declaration. simpl.
+repeat setoid_rewrite bind_ret_.
+repeat setoid_rewrite bind_bind.
+repeat setoid_rewrite bind_ret_.
+unfold endo. unfold Endo_id. 
+reflexivity.
+Qed.
+
+
+Lemma unfold_iter {E A B} (f : A -> itree E (A + B)) (x : A) :
+  (ITree.iter f x) ≈ ITree.bind (f x) (fun lr => ITree.on_left lr l (Tau (ITree.iter f l))).
+Proof.
+  rewrite unfold_aloop_. reflexivity.
+Qed.
+
+(* Lemma eq_what : (Eqv.eqv (Name "entry") (Name "entry")) -> (if Eqv.eqv_dec_p (Name "entry") (Name "entry") then true else false) = true.
+Proof.
+pose Eqv.eqv (Name "entry") (Name "entry")
+*)
+
+Lemma eq_entry : (if Eqv.eqv_dec_p (Name "entry") (Name "entry") then true else false) = true.
+Proof.
+destruct Eqv.eqv_dec_p.
+ + reflexivity.
+ + contradict n. reflexivity.
+Qed. 
+
+(* Lemma empty_iter : 
+ITree.iter
+             (fun '(bid_from, bid_src) =>
+              match
+                (if if Eqv.eqv_dec_p (Name "entry") bid_src then true else false
+                 then
+                  Some
+                    (tfmap (typ_to_dtyp [])
+                       {|
+                         blk_id := Name "entry";
+                         blk_phis := [];
+                         blk_code := [];
+                         blk_term := TERM_Ret (TYPE_I 32, EXP_Integer 1%Z);
+                         blk_comments := None
+                       |})
+                 else None)
+              with
+              | Some block_src =>
+                  bd <-
+                  ((dvs <- Util.map_monad (fun x : local_id * phi dtyp => translate exp_to_instr ⟦ x ⟧Φ (bid_from)) (blk_phis block_src);;
+                    Util.map_monad (fun '(id, dv) => trigger (LocalWrite id dv)) dvs;; Ret tt);;
+                   (Util.map_monad denote_instr (blk_code block_src);; Ret tt);; translate exp_to_instr ⟦ blk_term block_src ⟧t);;
+                  match bd with
+                  | inl bid_target => Ret (inl (bid_src, bid_target))
+                  | inr dv => Ret (inr (inr dv))
+                  end
+              | None => Ret (inr (inl (bid_from, bid_src)))
+              end) (Name "entry", Name "entry") ≈ Ret (inr (UVALUE_I32 (Int32.repr 1))) .
+Proof.
+setoid_rewrite unfold_iter.
+simpl.
+rewrite eq_entry. simpl. cbn.
+repeat setoid_rewrite bind_ret_.
+unfold exp_to_instr. simpl.
+unfold denote_exp . simpl. rewrite typ_to_dtyp_equation. unfold coerce_integer_to_int. simpl.
+repeat setoid_rewrite bind_ret_. rewrite unfold_translate . simpl. rewrite bind_ret_. rewrite bind_ret_.
+reflexivity.
+Qed.
+
+Lemma test_lemma1 : ⟦ tfmap (typ_to_dtyp []) [{| blk_id := Name "entry"; blk_phis := []; blk_code := []; blk_term := TERM_Ret (TYPE_I 32, EXP_Integer 1%Z); blk_comments := None |}] ⟧bs (Name "entry", Name "entry") ≈ Ret (inr (UVALUE_I32 (Int32.repr 1))).
+Proof.
+cbn. 
+unfold denote_ocfg. cbn. simpl. simpl_iter.
+setoid_rewrite empty_iter.
+reflexivity.
+Qed.
+
+Lemma test_lemma2 : r <-
+        ⟦ [tfmap (typ_to_dtyp [])
+             {|
+               blk_id := Name "entry";
+               blk_phis := [];
+               blk_code := [];
+               blk_term := TERM_Ret (TYPE_I 32, EXP_Integer 1%Z);
+               blk_comments := None
+             |}] ⟧bs (Name "entry", Name "entry");;
+        match r with
+        | inl bid => raise ("Can't find block in denote_cfg " ++ CeresSerialize.to_string (snd bid))
+        | inr uv => Ret uv
+        end ≈ Ret (UVALUE_I32 (Int32.repr 1)).
+Proof. 
+  rewrite test_lemma1. rewrite bind_ret_. reflexivity.
+Qed.
+
+Lemma test_lemma3 : translate instr_to_L0'
+       (r <-
+        ⟦ [tfmap (typ_to_dtyp [])
+             {|
+               blk_id := Name "entry";
+               blk_phis := [];
+               blk_code := [];
+               blk_term := TERM_Ret (TYPE_I 32, EXP_Integer 1%Z);
+               blk_comments := None
+             |}] ⟧bs (Name "entry", Name "entry");;
+        match r with
+        | inl bid => raise ("Can't find block in denote_cfg " ++ CeresSerialize.to_string (snd bid))
+        | inr uv => Ret uv
+        end) ≈ Ret (UVALUE_I32 (Int32.repr 1)).
+Proof.
+  unfold instr_to_L0'.
+  rewrite test_lemma2. cbn.
+  rewrite unfold_translate. simpl.
+  reflexivity.
+Qed.
+
+Lemma test_lemma4 : rv <-
+     translate instr_to_L0'
+       (r <-
+        ⟦ [tfmap (typ_to_dtyp [])
+             {|
+               blk_id := Name "entry";
+               blk_phis := [];
+               blk_code := [];
+               blk_term := TERM_Ret (TYPE_I 32, EXP_Integer 1%Z);
+               blk_comments := None
+             |}] ⟧bs (Name "entry", Name "entry");;
+        match r with
+        | inl bid => raise ("Can't find block in denote_cfg " ++ CeresSerialize.to_string (snd bid))
+        | inr uv => Ret uv
+        end);; trigger StackPop;; trigger MemPop;; Ret rv ≈ trigger StackPop;; trigger MemPop;; Ret (UVALUE_I32 (Int32.repr 1)).
+Proof.
+rewrite test_lemma3.
+setoid_rewrite bind_ret_.
+reflexivity.
+Qed.
+
+(* Lemma test_lemma5 : (fun args : list uvalue =>
+       bs <-
+       lift_err (fun x0 : list (local_id * uvalue) => Ret x0) match args with
+                                                              | [] | _ => inr []
+                                                              end;;
+       trigger MemPush;;
+       trigger (StackPush (map (fun '(k, v) => (k, v)) bs));;
+       rv <-
+       translate instr_to_L0'
+         (r <-
+          ⟦ [tfmap (typ_to_dtyp [])
+               {|
+                 blk_id := Name "entry";
+                 blk_phis := [];
+                 blk_code := [];
+                 blk_term := TERM_Ret (TYPE_I 32, EXP_Integer 1%Z);
+                 blk_comments := None
+               |}] ⟧bs (Name "entry", Name "entry");;
+          match r with
+          | inl bid => raise ("Can't find block in denote_cfg " ++ CeresSerialize.to_string (snd bid))
+          | inr uv => Ret uv
+          end);; trigger StackPop;; trigger MemPop;; Ret rv) [] ≈ Ret (UVALUE_I32 (Int32.repr 1)). *)
+
+Ltac pose_interp3_alloca m' a' A AE:=
+  match goal with
+  | [|-context[ℑs3 (trigger (Alloca ?t)) ?g ?l ?m]] =>
+    pose proof (interp3_alloca
+                  m t g l)
+      as [m' [a' [A AE]]]
+  end. *)
+
+Locate resum.
+Locate pat.
+
+(* Lemma test2 : State.interp_state (interp_local_stack_h (handle_local (v:=uvalue))) (SemNotations.Ret1 [] 1) (nil, nil) = Ret tt. *)
+
+(* Lemma test : interp_mcfg3  (trigger (Alloca DTYPE_Pointer);; Ret tt) [] ([],[]) empty_memory_stack ≈
+ Ret (empty_memory_stack, (nil, nil, (nil, tt))) .
+Proof.
+unfold interp_mcfg3.
+MCFGTactics.go.
+rewrite interp_memory_trigger. cbn.
+rewrite bind_bind. cbn.
+unfold lift_pure_err, lift_err.
+unfold allocate. cbn.
+MCFGTactics.go.
+unfold concrete_empty, make_empty_logical_block.
+reflexivity.
+
+setoid_rewrite interp_memory_ret  .
+vred_E3.
+
+setoid_rewrite interp_intrinsics_bind_trigger. cbn.
+setoid_rewrite interp_intrinsics_ret. simpl.
+unfold resum.
+unfold ReSum_inr.
+unfold resum.
+unfold ReSum_inl.
+unfold resum.
+unfold ReSum_id.
+unfold id_.
+unfold Id_IFun.
+simpl.
+unfold cat, Cat_IFun. unfold inl_, inr_.
+unfold Inr_sum1, Inl_sum1.
+setoid_rewrite interp_global_bind_trigger. cbn.
+setoid_rewrite interp_global_ret.
+setoid_rewrite interp_local_stack_bind.
+setoid_rewrite interp_local_stack_bind.
+setoid_rewrite interp_local_stack_trigger. cbn.
+unfold interp_local_stack. simpl. unfold interp_local_stack_h. simpl.
+
+repeat setoid_rewrite interp_memory_bind  .
+setoid_rewrite interp_memory_trigger. cbn. simpl. cbn. simpl.
+repeat setoid_rewrite bind_ret_. 
+setoid_rewrite interp_memory_ret.
+repeat setoid_rewrite bind_ret_. simpl.
+
+repeat setoid_rewrite interp_state_ret.
+setoid_rewrite bind_ret_. cbn.
+unfold interp_memory. simpl.
+unfold interp_memory_h. simpl.
+
+setoid_rewrite interp_memory_bind.
+
+
+unfold ReSum_inr. cbn.
+
+
+setoid_rewrite interp3_bind .
+setoid_rewrite interp3_alloca.
+pose (t := DTYPE_Pointer).
+unfold non_void in H.
+assert (non_void DTYPE_Pointer).
+{
+unfold non_void.
+f_equal. 
+
+}
+assert (H_pointer : exists (m' : memory_stack) (a' : addr),
+            allocate empty_memory_stack DTYPE_Pointer = inr (m', a') /\
+            ℑs3 (trigger (Alloca DTYPE_Pointer)) [] ([], []) empty_memory_stack ≈
+            ret (m', ([], ([] , DVALUE_Addr a')))). *)
+
+Lemma denote_simpl : (denote_mcfg
+              [(DVALUE_Addr (0%Z, 0%Z),
+               ⟦ tfmap (typ_to_dtyp [])
+                   {|
+                     df_prototype :=
+                       {|
+                         dc_name := Name "main";
+                         dc_type := TYPE_Function (TYPE_I 32) [];
+                         dc_param_attrs := ([], []);
+                         dc_linkage := None;
+                         dc_visibility := None;
+                         dc_dll_storage := None;
+                         dc_cconv := None;
+                         dc_attrs := [];
+                         dc_section := None;
+                         dc_align := None;
+                         dc_gc := None
+                       |};
+                     df_args := [];
+                     df_instrs :=
+                       cfg_of_definition typ
+                         {|
+                           df_prototype :=
+                             {|
+                               dc_name := Name "main";
+                               dc_type := TYPE_Function (TYPE_I 32) [];
+                               dc_param_attrs := ([], []);
+                               dc_linkage := None;
+                               dc_visibility := None;
+                               dc_dll_storage := None;
+                               dc_cconv := None;
+                               dc_attrs := [];
+                               dc_section := None;
+                               dc_align := None;
+                               dc_gc := None
+                             |};
+                           df_args := [];
+                           df_instrs :=
+                             ({|
+                                blk_id := Name "entry"; blk_phis := []; blk_code := []; blk_term := TERM_Ret (TYPE_I 32, EXP_Integer 1%Z); blk_comments := None
+                              |}, [])
+                         |}
+                   |} ⟧f)] (DTYPE_I 32) (dvalue_to_uvalue (DVALUE_Addr (0%Z, 0%Z))) []) ≈ Ret (UVALUE_I32 (repr 1)).
+Proof.
+unfold denote_mcfg.
+unfold mrec.
+repeat setoid_rewrite bind_ret_. 
+unfold lookup_defn. simpl.
+unfold dvalue_eq_dec.
+unfold dvalue_to_uvalue. simpl.
+
+
+
+Theorem empty_th : ℑs3 e_test [] ([],[]) empty_memory_stack  ≈ Ret (empty_memory_stack, (nil, nil, (nil,  (UVALUE_I32 (repr 1))))).
+Proof.
+unfold e_test. unfold denote_vellvm.
+rewrite empty_env.
+unfold ℑs3. cbn.
+MCFGTactics.go.
+rewrite interp_memory_trigger. cbn. unfold lift_pure_err. simpl. cbn. setoid_rewrite bind_ret_. setoid_rewrite bind_ret_.
+rewrite interp_memory_ret. setoid_rewrite bind_ret_.
+rewrite interp_local_stack_ret.
+rewrite interp_memory_ret. setoid_rewrite bind_ret_.
+MCFGTactics.go.
+unfold denote_mcfg. simpl.
+
+
+
+rewrite ITree.Interp.RecursionFacts.mrec_as_interp.
+rewrite unfold_interp. unfold _interp. simpl. unfold concretize_or_pick.
+
+Import DenoteTactics.
+setoid_rewrite bind_bind    .
+
+unfold cfg_of_definition. simpl.
+unfold address_one_function. simpl.
+unfold denote_function. simpl.
+unfold denote_cfg. simpl. cbn.
+unfold endo. unfold Endo_id.
+unfold ℑs3.
+MCFGTactics.go.
+repeat rewrite interp_memory_trigger. cbn.
+rewrite bind_bind. cbn.
+unfold lift_pure_err, lift_err.
+unfold allocate. cbn.
+MCFGTactics.go.
+unfold interp_memory.
+unfold interp_local_stack. cbn.
+rewrite unfold_interp_state.
+unfold _interp_state. cbn.
+unfold interp_local_stack_h.
+simpl.
+
+
+auto.
+setoid_rewrite interp3_bind_trigger .
+pose_interp3_alloca.
+setoid_rewrite bind_trigger.
+setoid_rewrite interp1_ret. 
+setoid_rewrite test_lemma4.
+setoid_rewrite bind_ret_. rewrite bind_trigger. setoid_rewrite bind_trigger. cbn. setoid_rewrite test_lemma.
+rewrite empty_iter.
+setoid_rewrite unfold_iter.
+
+
+unfold convert_types. unfold mcfg_of_tle. unfold mcfg_of_modul. simpl.
+repeat setoid_rewrite bind_ret_.
+unfold build_global_environment.
+simpl. cbn.
+repeat setoid_rewrite bind_ret_.
+unfold denote_function. unfold denote_cfg.
+simpl. cbn.
+setoid_rewrite bind_vis. setoid_rewrite bind_vis. setoid_rewrite bind_vis. repeat setoid_rewrite bind_ret_. repeat setoid_rewrite bind_bind. repeat setoid_rewrite bind_ret_. cbn.
+setoid_rewrite translate_ret. repeat setoid_rewrite bind_ret_.
+unfold denote_ocfg. simpl. cbn. simpl.
+give_up.
+Admitted.
+
+
+
+Definition empty_cfg : cfg dtyp :=
+{|
+  init := Anon 0%Z;
+  blks := nil;
+  args := nil;
+|}.
+
+Definition empty_dec : declaration dtyp :=
+{|
+  dc_name        := Anon 1%Z;
+  dc_type        := (DTYPE_I 32%N) ;    (* INVARIANT: should be TYPE_Function (ret_t * args_t) *)
+  dc_param_attrs := (nil, nil); (* ret_attrs * args_attrs *)
+  dc_linkage     := None;
+  dc_visibility  := None;
+  dc_dll_storage := None;
+  dc_cconv       := None;
+  dc_attrs       := nil;
+  dc_section     := None;
+  dc_align       := None;
+  dc_gc          := None;
+|}.
+
+Definition empty_def : definition dtyp (cfg dtyp) :=
+{|
+  df_prototype   := empty_dec;
+  df_args        := nil;
+  df_instrs      := empty_cfg;
+|}.
+
+
+Definition empty_fun : function_denotation :=
+  denote_function empty_def.
+
+ Definition empty_mcfg : itree L0 uvalue :=
+  denote_mcfg [((DVALUE_I32 (repr 0)), empty_fun)] (DTYPE_I 32%N) (UVALUE_I32 (repr 0)) nil. 
+
+Check dvalue_eq_dec (d1:=DVALUE_I32 (Int32.repr 0))
+         (d2:=DVALUE_I32 (Int32.repr 0)).
+
+Lemma equals : 
+DVALUE_I32 (Int32.repr 0) = DVALUE_I32 (Int32.repr 0).
+Proof.
+reflexivity.
+Qed.
+
+Lemma test : (if
+      if
+       dvalue_eq_dec (d1:=DVALUE_I32 (Int32.repr 0))
+         (d2:=DVALUE_I32 (Int32.repr 0))
+      then true
+      else false
+     then Some empty_fun
+     else None)  = Some empty_fun.
+Proof.
+  pose proof equals as Hequals.
+  destruct dvalue_eq_dec as [Heq | Hneq].
+    - reflexivity.
+    - contradiction.
+Qed.
+
+Lemma fun_empty : empty_fun [] ≈ Ret (UVALUE_I32 (repr 0)).
+Proof.
+unfold empty_fun.
+unfold denote_function. simpl.
+give_up.
+Admitted.
+(* 
+Definition dirty_tree {E:Type->Type} {T:Type} : itree (CallE +' ExternalCallE +' E) unit :=
+  Ret tt.
+
+Definition clean_tree {E:Type->Type} {T:Type}  : itree (ExternalCallE +' E) unit :=
+  Ret tt.
+
+(* The term "dirty_tree" has type "itree (CallE +' ExternalCallE) unit" while it is expected to have type
+ "forall T : Type, CallE T -> itree (CallE +' ExternalCallE +' ?E2) T". *)
+
+
+Definition empty_conv {E:Type->Type} : forall T : Type, CallE T -> itree (ExternalCallE +' E) T :=
+fun T call => clean_tree.
+
+
+Definition easy_rec :=
+        @mrec CallE (ExternalCallE +' _) dirty_tree unit.
+ *)
+
+             
+
+
+Lemma test1 : denote_ocfg [] (Anon 0%Z, Anon 0%Z) ≈ Ret (inl (Anon 0%Z, Anon 0%Z)).
+Proof.
+setoid_rewrite denote_ocfg_nil.
+reflexivity.
+Qed.
+
+Theorem empty_th2 : empty_mcfg ≈ Ret (UVALUE_I32 (repr 0)).
+Proof.
+unfold empty_mcfg.
+unfold denote_mcfg.
+simpl.
+unfold concretize_or_pick. simpl.
+unfold mrec. simpl.
+repeat setoid_rewrite bind_ret_. simpl.
+pose proof equals as Hequals.
+rewrite test. setoid_rewrite unfold_interp_mrec.
+unfold _interp_mrec. cbn. simpl. repeat setoid_rewrite bind_ret_.  setoid_rewrite unfold_interp_mrec. unfold _interp_mrec. cbn. setoid_rewrite unfold_interp_mrec. unfold _interp_mrec. cbn. setoid_rewrite test1.
+unfold denote_ocfg. simpl. unfold iter.
+ setoid_rewrite bind_ret_r_.
+
+
+
+ unfold empty_fun. unfold empty_def. unfold denote_function. simpl. repeat setoid_rewrite bind_ret_. simpl.
+unfold mrecursive. simpl.
+apply Proper_interp_mrec .
+
+unfold dvalue_to_uvalue.
+rewrite interp_mrecursive.
