src/Extraction.v
@@ -1,5 +1,5 @@
 From ASL Require Import
- Ast Compiler.
+ Ast Compiler Correctness.
 From Coq Require Import
  Extraction String.
 
