src/InterpretMemoryTest.v
@@ -1,0 +1,135 @@
+From Vellvm Require Import
+Semantics Syntax TopLevel Theory Utils.PropT. 
+
+From ITree Require Import
+  ITree ITreeFacts KTree KTreeFacts Events.StateFacts Events.State.
+
+From ExtLib Require Import
+RelDec Tactics.
+
+From Coq Require Import
+ZArith List String Classes.RelationClasses.
+
+Import ITreeNotations.
+Import ListNotations.
+Import SemNotations.
+
+Open Scope list_scope.
+Open Scope string_scope.
+
+
+
+Local Ltac pose_interp3_alloca m' a' A AE:=
+  match goal with
+  | [|-context[ℑ3  (trigger (Alloca ?t)) ?g ?l ?m]] =>
+    pose proof (interp_cfg3_alloca
+                  m t g l)
+      as [m' [a' [A AE]]]
+  end.
+
+Locate add.
+
+(* Lemma simpl_mem : (concrete_empty, add 0%Z (make_empty_logical_block (DTYPE_I 32)) logical_empty, Singleton [0%Z]) = ([], ([],[])).
+ *)
+Theorem alloca_test : ℑ3 (trigger (Alloca (DTYPE_I 32));;Ret (UVALUE_I32 (repr 1))) [] [] empty_memory_stack ≈
+ Ret3 [] [] (concrete_empty, add 0%Z (make_empty_logical_block (DTYPE_I 32)) logical_empty, Singleton [0%Z])  (UVALUE_I32 (Int32.repr 1)).
+Proof.
+  rewrite interp_cfg3_bind.
+  pose_interp3_alloca m' a' A AE.
+    + unfold non_void.
+      discriminate.
+    + rewrite AE.
+      cbn.
+      rewrite bind_ret_.
+      rewrite interp_cfg3_ret.
+      apply allocate_inv in A.
+      cbn in A.
+      destruct A. destruct H0.
+      rewrite H1 in AE.
+      rewrite H0.
+      reflexivity.
+Qed.
+
+Theorem alloca_simpl : forall x, ℑ3 (denote_instr (IId (Name x), (INSTR_Alloca (DTYPE_I 32%N) None None))) [] [] empty_memory_stack ≈
+Ret3 [] (FMapAList.alist_add (Name x) (UVALUE_Addr (0%Z, 0%Z)) [])
+  (concrete_empty, add 0%Z (make_empty_logical_block (DTYPE_I 32)) logical_empty,
+  Singleton [0%Z]) tt.
+Proof.
+  intros.
+  unfold denote_instr.
+  cbn.
+  rewrite interp_cfg3_bind.
+  pose_interp3_alloca m' a' A AE.
+    + unfold non_void.
+      discriminate.
+    + rewrite AE.
+      apply allocate_inv in A.
+      cbn in A.
+      destruct A. destruct H0.
+      rewrite H1 in AE.
+      rewrite H0, H1.
+      rewrite bind_ret_.
+      cbn.
+      clear m' a' H H0 H1 AE.
+      rewrite interp_cfg3_LW.
+      cbn.   
+      reflexivity.
+Qed.
+
+Definition gen_alloca_ins (x:string) := (IId (Name x), (INSTR_Alloca (DTYPE_I 32%N) None None)).
+Definition gen_store_ins (x:string) (v:int) := (IVoid 0%Z, (INSTR_Store false ((DTYPE_I 32%N), (EXP_Integer (v)%Z)) (DTYPE_Pointer, (EXP_Ident (ID_Local (Name x)))) None)).
+
+Lemma interp_cfg3_concretize_or_pick_concrete :
+  forall (uv : uvalue) (dv : dvalue) P g l m,
+    is_concrete uv ->
+    uvalue_to_dvalue uv = inr dv ->
+    ℑ3 (concretize_or_pick uv P) g l m ≈ Ret3 g l m dv.
+Proof.
+  intros * CONC CONV.
+  unfold concretize_or_pick.
+  rewrite CONC.
+  cbn.
+  unfold lift_err.
+  rewrite CONV.
+  rewrite interp_cfg3_ret.
+  reflexivity.
+Qed.
+
+
+
+Theorem x_eq_5 : ℑ3 (denote_code [(gen_alloca_ins "x") ; (gen_store_ins "x" 5%Z)]) [] [] empty_memory_stack ≈ Ret (empty_memory_stack, ((FMapAList.alist_add (Name "x") (UVALUE_Addr (0%Z, 0%Z)) []), ([], tt))).
+Proof.
+rewrite denote_code_cons.
+rewrite interp_cfg3_bind.
+unfold gen_alloca_ins.
+rewrite alloca_simpl. 
+rewrite bind_ret_.
+rewrite denote_code_singleton.
+unfold gen_store_ins.
+
+cbn.
+rewrite translate_ret.
+rewrite bind_ret_.
+rewrite interp_cfg3_bind.
+assert(H: forall g l m, ℑ3 (concretize_or_pick (UVALUE_I32 (Int32.repr 5)) True) g l m ≈ Ret (m, (l, (g, DVALUE_I32 (repr 5))))).
+  + intros.
+    unfold concretize_or_pick.
+    cbn.
+    unfold lift_err.
+    rewrite interp_cfg3_ret.
+    reflexivity.
+  + rewrite H; clear H.
+rewrite bind_ret_.
+repeat rewrite translate_trigger.
+ExpTactics.simplify_translations.
+rewrite interp_cfg3_bind.
+assert(H: Maps.lookup (Name "x") (FMapAList.alist_add (Name "x") (UVALUE_Addr (0%Z, 0%Z)) []) = Some (UVALUE_Addr (0%Z, 0%Z))).
+  - reflexivity.
+  - pose proof interp_cfg3_LR.
+    ExpTactics.step.
+    clear H H0.
+cbn.
+rewrite bind_ret_.
+InstrTactics.step.
+  -- reflexivity.
+  -- unfold write. simpl.
